DeBruijnSSA/BinSyntax/Rewrite/Region/Compose/Seq.lean
@@ -197,13 +197,94 @@ theorem Eqv.let2_seq {Γ : Ctx α ε} {L : LCtx α}
   : (Eqv.let2 a r) ;; s = Eqv.let2 a (r ;; s.vwk1.vwk1) := by
   simp only [seq_def, lsubst_let2, Subst.Eqv.vliftn₂_eq_vlift_vlift, vlift_alpha0]
 
--- theorem Eqv.seq_let2_wk0_vwk2 {Γ : Ctx α ε} {L : LCtx α}
---   (r : Eqv φ (⟨X, ⊥⟩::Γ) (Y::L))
---   (a : Term.Eqv φ Γ ⟨A.prod B, ⊥⟩)
---   (s : Eqv φ (⟨B, ⊥⟩::⟨A, ⊥⟩::Γ) (D::L))
---   : (r ;; let2 a.wk0 s.vwk2) = let2 a.wk0
---     (let1 (Term.Eqv.var 2 Ctx.Var.shead.step.step) (r.vwk1.vwk1.vwk1 ;; s.vwk2.vwk0)) := by
---   sorry
+theorem Eqv.seq_let1_wk0_pure {Γ : Ctx α ε} {L : LCtx α}
+  (a : Term.Eqv φ Γ ⟨X, ⊥⟩)
+  (r : Eqv φ (⟨A, ⊥⟩::Γ) (B::L)) (s : Eqv φ (⟨X, ⊥⟩::⟨B, ⊥⟩::Γ) (C::L))
+  : r ;; (let1 a.wk0 s) = let1 a.wk0 (r.vwk1 ;; s.vswap01).vswap01 := by
+  simp only [seq_def, let1_beta]
+  induction a using Quotient.inductionOn
+  induction r using Quotient.inductionOn
+  induction s using Quotient.inductionOn
+  apply Eqv.eq_of_reg_eq
+  simp only [Set.mem_setOf_eq, InS.coe_lsubst, InS.coe_alpha0, InS.coe_vwk, Ctx.InS.coe_wk1,
+    InS.coe_vsubst, Term.InS.coe_subst0, Term.InS.coe_wk, Ctx.InS.coe_wk0, Ctx.InS.coe_swap01,
+    vwk_lsubst, Region.vsubst_lsubst]
+  congr
+  · funext k; cases k with
+    | zero =>
+      simp only [alpha, Function.update_same, Region.vwk_vwk, Function.comp_apply]
+      simp only [<-Region.vsubst_fromWk, Region.vsubst_vsubst]
+      congr
+      funext k; cases k using Nat.cases2 with
+      | zero => simp only [Term.Subst.comp, Term.subst0_zero, Term.subst_fromWk, Term.wk_wk,
+        Nat.liftWk_succ_comp_succ, Term.subst, Function.comp_apply, Nat.swap0_0, Nat.liftWk_succ,
+        Nat.succ_eq_add_one, zero_add, Nat.reduceAdd, zero_lt_one, Nat.swap0_lt,
+        Term.Subst.lift_succ]; rfl
+      | _ => rfl
+    | succ => rfl
+  · rw [Region.vwk_vwk, <-Region.vsubst_fromWk, Region.vsubst_vsubst, Region.vsubst_id']
+    funext k; cases k <;> rfl
+
+-- theorem Eqv.lsubst_let2_alpha0 {Γ : Ctx α ε} {L : LCtx α}
+--   (p : Term.Eqv φ Γ ⟨X.prod Y, ⊥⟩)
+--   (r : Eqv φ (⟨A, ⊥⟩::Γ) (B::L)) (s : Eqv φ (⟨Y, ⊥⟩::⟨X, ⊥⟩::⟨B, ⊥⟩::⟨A, ⊥⟩::Γ) (C::L))
+--   : lsubst (let2 p.wk0.wk0 s).alpha0 r
+--   = let2 p.wk0 (lsubst (alpha0 s.vswap02.vswap02) r.vwk0.vwk0)
+--   := by induction r using Eqv.arrow_induction with
+--   | br ℓ a hℓ =>
+--     cases ℓ with
+--     | zero =>
+--       induction p using Quotient.inductionOn
+--       induction s using Quotient.inductionOn
+--       induction a using Quotient.inductionOn
+--       apply Eqv.eq_of_reg_eq
+--       simp only [Set.mem_setOf_eq, InS.lsubst_br, List.length_cons, List.get_eq_getElem,
+--         InS.coe_vsubst, Term.InS.coe_subst0, InS.coe_vwk_id, Subst.InS.coe_get, InS.coe_alpha0,
+--         InS.coe_let2, Term.InS.coe_wk, Ctx.InS.coe_wk0, InS.vwk_br, InS.coe_vwk, Ctx.InS.coe_swap02]
+--       simp only [Region.vsubst, Term.wk_succ_subst_subst0, alpha, ← vsubst_fromWk,
+--         Region.vsubst_vsubst, Function.update_same, let2.injEq, true_and]
+--       congr
+--       funext k; cases k using Nat.cases3 with
+--       | two => simp only [Term.Subst.liftn, lt_self_iff_false, ↓reduceIte, le_refl,
+--         tsub_eq_zero_of_le, Term.subst0_zero, Term.Subst.comp, Term.subst, Term.wk_wk,
+--         Nat.one_lt_ofNat, Nat.swap0_lt, Nat.ofNat_pos]; rfl
+--       | _ => rfl
+--     | succ ℓ => simp [get_alpha0, let2_br, Term.Eqv.nil, Term.Eqv.let2_wk0_wk0_pure]
+--   | let1 a r => sorry
+--   | let2 a r => sorry
+--   | case a l r => sorry
+--   | cfg R β G => sorry
+
+theorem Eqv.seq_let2_wk0_pure {Γ : Ctx α ε} {L : LCtx α}
+  {a : Term.Eqv φ Γ ⟨X.prod Y, ⊥⟩}
+  {r : Eqv φ (⟨A, ⊥⟩::Γ) (B::L)} {s : Eqv φ (⟨Y, ⊥⟩::⟨X, ⊥⟩::⟨B, ⊥⟩::Γ) (C::L)}
+  : r ;; (let2 a.wk0 s) = let2 a.wk0 (r.vwk1.vwk1 ;; s.vswap02.vswap02).vswap02 := by
+  sorry
+  -- rw [seq, vwk1_let2, Term.Eqv.wk0_wk1, lsubst_let2_alpha0]
+  -- congr
+  -- rw [seq]
+  -- induction r using Quotient.inductionOn
+  -- induction s using Quotient.inductionOn
+  -- induction a using Quotient.inductionOn
+  -- apply Eqv.eq_of_reg_eq
+  -- simp only [Set.mem_setOf_eq, InS.coe_lsubst, InS.coe_alpha0, InS.coe_vwk, Ctx.InS.coe_swap02,
+  --   Ctx.InS.coe_wk3, Ctx.InS.coe_wk0, Ctx.InS.coe_wk1, vwk_lsubst]
+  -- congr 1
+  -- · funext k; cases k with
+  --   | zero =>
+  --     simp only [alpha, Region.vwk_vwk, Function.update_same, Function.comp_apply]
+  --     congr
+  --     funext k; cases k using Nat.cases3 <;> rfl
+  --   | succ => rfl
+  -- · simp only [Region.vwk_vwk]; congr; funext k; cases k <;> rfl
+
+theorem Eqv.seq_let2_wk0_pure' {Γ : Ctx α ε} {L : LCtx α}
+  {a : Term.Eqv φ (_::Γ) ⟨X.prod Y, ⊥⟩} {a' : Term.Eqv φ Γ ⟨X.prod Y, ⊥⟩}
+  {r : Eqv φ (⟨A, ⊥⟩::Γ) (B::L)} {s : Eqv φ (⟨Y, ⊥⟩::⟨X, ⊥⟩::⟨B, ⊥⟩::Γ) (C::L)}
+  (ha : a = a'.wk0)
+  : r ;; (let2 a s) = let2 a'.wk0 (r.vwk1.vwk1 ;; s.vswap02.vswap02).vswap02 := by
+  cases ha; rw [seq_let2_wk0_pure]
+
 
 theorem Eqv.case_seq {Γ : Ctx α ε} {L : LCtx α}
   (a : Term.Eqv φ (⟨A, ⊥⟩::Γ) ⟨X.coprod Y, e⟩)
